proof/access-control/AARCH64/ArchDomainSepInv.thy
@@ -56,7 +56,8 @@ crunch handle_vm_fault, handle_vm_fault, perform_pg_inv_unmap,
        perform_pg_inv_get_addr, perform_pt_inv_map, perform_pt_inv_unmap,
        handle_arch_fault_reply, arch_mask_irq_signal, arch_switch_to_thread,
        arch_switch_to_idle_thread, arch_activate_idle_thread, store_asid_pool_entry,
-       arch_prepare_set_domain, arch_prepare_next_domain, arch_post_set_flags
+       arch_prepare_set_domain, arch_prepare_next_domain, arch_post_set_flags,
+       handle_spurious_irq
   for domain_sep_inv[DomainSepInv_assms, wp]: "domain_sep_inv irqs st"
   (wp: crunch_wps)
 
