proof/invariant-abstract/ARM/ArchDetSchedDomainTime_AI.thy
@@ -104,13 +104,13 @@ lemma handle_interrupt_valid_domain_time [DetSchedDomainTime_AI_assms]:
    apply wpsimp+
   done
 
-crunch handle_reserved_irq
+crunch handle_reserved_irq, handle_spurious_irq
   for domain_time_inv[wp, DetSchedDomainTime_AI_assms]: "\<lambda>s. P (domain_time s)"
+  and domain_list_inv[wp, DetSchedDomainTime_AI_assms]: "\<lambda>s. P (domain_list s)"
   (wp: crunch_wps mapM_wp subset_refl simp: crunch_simps)
 
-crunch handle_reserved_irq
-  for domain_list_inv[wp, DetSchedDomainTime_AI_assms]: "\<lambda>s. P (domain_list s)"
-  (wp: crunch_wps mapM_wp subset_refl simp: crunch_simps)
+crunch handle_spurious_irq
+  for scheduler_action[wp, DetSchedDomainTime_AI_assms]: "\<lambda>s. P (scheduler_action s)"
 
 end
 
