proof/invariant-abstract/RISCV64/ArchDetSchedSchedule_AI.thy
@@ -327,9 +327,9 @@ crunch arch_switch_to_thread
   for etcbs_of[wp, DetSchedSchedule_AI_assms]: "\<lambda>s. P (etcbs_of s)"
   and cur_domain[wp, DetSchedSchedule_AI_assms]: "\<lambda>s. P (cur_domain s)"
 
-crunch arch_switch_to_thread
-  for etcbs_of[wp, DetSchedSchedule_AI_assms]: "\<lambda>s. P (etcbs_of s)"
-  and cur_domain[wp, DetSchedSchedule_AI_assms]: "\<lambda>s. P (cur_domain s)"
+crunch handle_spurious_irq
+  for valid_sched[wp, DetSchedSchedule_AI_assms]: valid_sched
+  and valid_idle[wp, DetSchedSchedule_AI_assms]: valid_idle
 
 end
 
