proof/invariant-abstract/Syscall_AI.thy
@@ -1361,19 +1361,13 @@ lemma select_insert:
 context Syscall_AI begin
 
 lemma he_invs[wp]:
-  "\<And>e.
-    \<lbrace>\<lambda>s. invs s \<and> (e \<noteq> Interrupt \<longrightarrow> ct_active s)\<rbrace>
-      handle_event e
-    \<lbrace>\<lambda>rv. invs :: 'state_ext state \<Rightarrow> bool\<rbrace>"
-  apply (case_tac e, simp_all)
-      apply (rename_tac syscall)
-      apply (case_tac syscall, simp_all)
-      apply (((rule hoare_pre, wp hvmf_active hr_invs  ) |
-                 wpc | wp hoare_drop_imps hoare_vcg_all_lift |
-                 simp add: if_apply_def2 |
-                 fastforce simp: tcb_at_invs ct_in_state_def valid_fault_def
-                         elim!: st_tcb_ex_cap)+)
-  done
+  "\<lbrace>\<lambda>s. invs s \<and> (e \<noteq> Interrupt \<longrightarrow> ct_active s)\<rbrace>
+   handle_event e
+   \<lbrace>\<lambda>rv. invs :: 'state_ext state \<Rightarrow> bool\<rbrace>"
+  by (case_tac e;
+      wpsimp wp: handle_spurious_irq_invs hvmf_active hr_invs;
+      fastforce simp: tcb_at_invs ct_in_state_def valid_fault_def
+                elim!: st_tcb_ex_cap)
 
 end
 
