proof/refine/AARCH64/Refine.thy
@@ -256,14 +256,11 @@ lemma schedule_sched_act_rct[wp]:
   by (wpsimp)
 
 lemma call_kernel_sched_act_rct[wp]:
-  "\<lbrace>einvs and (\<lambda>s. e \<noteq> Interrupt \<longrightarrow> ct_running s)
-     and (\<lambda>s. scheduler_action s = resume_cur_thread)\<rbrace>
-  call_kernel e
-  \<lbrace>\<lambda>rs (s::det_state). scheduler_action s = resume_cur_thread\<rbrace>"
-  apply (simp add: call_kernel_def)
-  apply (wp activate_thread_sched_act | simp)+
-  apply (clarsimp simp: active_from_running)
-  done
+  "\<lbrace>einvs and (\<lambda>s. e \<noteq> Interrupt \<longrightarrow> ct_running s) and (\<lambda>s. scheduler_action s = resume_cur_thread)\<rbrace>
+   call_kernel e
+   \<lbrace>\<lambda>rs (s::det_state). scheduler_action s = resume_cur_thread\<rbrace>"
+  unfolding call_kernel_def
+  by (wpsimp wp: activate_thread_sched_act handle_spurious_irq_invs simp: active_from_running)
 
 lemma kernel_entry_invs:
   "\<lbrace>einvs and (\<lambda>s. e \<noteq> Interrupt \<longrightarrow> ct_running s)
@@ -390,26 +387,19 @@ lemma dmo_getActiveIRQ_notin_non_kernel_IRQs[wp]:
   unfolding doMachineOp_def
   by (wpsimp simp: getActiveIRQ_def in_monad split: if_split_asm)
 
-lemma non_kernel_IRQs_strg:
-  "invs' s \<and> irq \<notin> Some ` non_kernel_IRQs \<and> Q \<Longrightarrow>
-    (\<exists>y. irq = Some y) \<longrightarrow> invs' s \<and> (the irq \<in> non_kernel_IRQs \<longrightarrow> P) \<and> Q"
-  by auto
-
 lemma ckernel_invs:
-  "\<lbrace>invs' and
-               (\<lambda>s. e \<noteq> Interrupt \<longrightarrow> ct_running' s) and
-               (\<lambda>s. ksSchedulerAction s = ResumeCurrentThread)\<rbrace>
-  callKernel e
-  \<lbrace>\<lambda>rs. (\<lambda>s. ksSchedulerAction s = ResumeCurrentThread)
+  "\<lbrace>invs' and (\<lambda>s. e \<noteq> Interrupt \<longrightarrow> ct_running' s) and
+    (\<lambda>s. ksSchedulerAction s = ResumeCurrentThread)\<rbrace>
+   callKernel e
+   \<lbrace>\<lambda>rs. (\<lambda>s. ksSchedulerAction s = ResumeCurrentThread)
     and (invs' and (ct_running' or ct_idle'))\<rbrace>"
-  apply (simp add: callKernel_def)
-  apply (rule hoare_pre)
-   apply (wp activate_invs' activate_sch_act schedule_sch
-             schedule_sch_act_simple he_invs' schedule_invs' hoare_vcg_if_lift3
-             hoare_drop_imp[where Q'="\<lambda>_. kernelExitAssertions"]
-          | simp add: no_irq_getActiveIRQ
-          | strengthen non_kernel_IRQs_strg[where Q=True, simplified], simp cong: conj_cong)+
-  done
+  unfolding callKernel_def
+  by (wpsimp wp: activate_invs' activate_sch_act schedule_sch
+                 schedule_sch_act_simple he_invs' schedule_invs' hoare_vcg_if_lift3
+                 hoare_drop_imp[where Q'="\<lambda>_. kernelExitAssertions"]
+                 hoare_drop_imp[where Q'="\<lambda>rv _. rv = None"]
+             simp: no_irq_getActiveIRQ
+      | strengthen non_kernel_IRQs_strg)+
 
 (* abstract and haskell have identical domain list fields *)
 abbreviation valid_domain_list' :: "'a kernel_state_scheme \<Rightarrow> bool" where
@@ -536,11 +526,6 @@ lemma None_drop:
   "P \<Longrightarrow> x = None \<longrightarrow> P"
   by simp
 
-lemma Ex_Some_conv:
-  "((\<exists>y. x = Some y) \<longrightarrow> P x) = (\<forall>y. x = Some y \<longrightarrow> P (Some y))"
-  by auto
-
-
 lemma kernel_corres':
   "corres dc (einvs and (\<lambda>s. event \<noteq> Interrupt \<longrightarrow> ct_running s) and (ct_running or ct_idle)
                and (\<lambda>s. scheduler_action s = resume_cur_thread))
@@ -549,53 +534,28 @@ lemma kernel_corres':
              (call_kernel event)
              (do _ \<leftarrow> runExceptT $
                       handleEvent event `~catchError~`
-                        (\<lambda>_. withoutPreemption $ do
-                               irq <- doMachineOp (getActiveIRQ True);
-                               when (isJust irq) $ handleInterrupt (fromJust irq)
-                             od);
+                        (\<lambda>_. withoutPreemption $ maybeHandleInterrupt True);
                  _ \<leftarrow> ThreadDecls_H.schedule;
                  activateThread
               od)"
-  unfolding call_kernel_def callKernel_def
-  apply (simp add: call_kernel_def callKernel_def)
-  apply (rule corres_guard_imp)
-    apply (rule corres_split)
-       apply (rule corres_split_handle[OF handleEvent_corres])
-         apply simp
-         apply (rule corres_split[OF corres_machine_op])
-            apply (rule corres_underlying_trivial)
-            apply (rule no_fail_getActiveIRQ)
-           apply clarsimp
-           apply (rule_tac x=irq in option_corres)
-            apply (rule_tac P=\<top> and P'=\<top> in corres_inst)
-            apply (simp add: when_def)
-           apply (rule corres_when[simplified dc_def], simp)
-           apply simp
-           apply (rule handleInterrupt_corres[simplified dc_def])
-          apply simp
-          apply (wpsimp wp: hoare_drop_imps hoare_vcg_all_lift simp: schact_is_rct_def)[1]
-         apply simp
-         apply (rule_tac Q'="\<lambda>irq s. invs' s \<and>
-                              (\<forall>irq'. irq = Some irq' \<longrightarrow>
-                                 intStateIRQTable (ksInterruptState s ) irq' \<noteq>
-                                 IRQInactive)"
-                      in hoare_post_imp)
-          apply simp
-         apply (wp doMachineOp_getActiveIRQ_IRQ_active handle_event_valid_sched | simp)+
-       apply (rule_tac Q'="\<lambda>_. \<top>" and E'="\<lambda>_. invs'" in hoare_strengthen_postE)
-         apply wpsimp+
-       apply (simp add: invs'_def valid_state'_def)
-      apply (rule corres_split[OF schedule_corres])
-        apply (rule activateThread_corres)
-       apply (wp schedule_invs' hoare_vcg_if_lift2 dmo_getActiveIRQ_non_kernel
-              | simp cong: rev_conj_cong | strengthen None_drop | subst Ex_Some_conv)+
+  unfolding call_kernel_def
+  apply (corres corres: handleEvent_corres corres_machine_op
+                        maybeHandleInterrupt_corres
+                simp: irq_state_independent_def
+         | corres_cases_both)+
+        apply (wpsimp wp: handle_event_valid_sched)+
+      apply (corres corres: schedule_corres activateThread_corres)
+      apply (wpsimp wp: schedule_invs' hoare_vcg_if_lift2 dmo_getActiveIRQ_non_kernel
+                        handle_spurious_irq_invs
+             | simp add: maybe_handle_interrupt_def cong: rev_conj_cong
+             | strengthen None_drop contract_all_imp_strg)+
      apply (rule_tac Q'="\<lambda>_. valid_sched and invs and valid_list" and
                      E'="\<lambda>_. valid_sched and invs and valid_list"
-            in hoare_strengthen_postE)
-       apply (wp handle_event_valid_sched hoare_vcg_imp_lift' |simp)+
-       apply (wp handle_event_valid_sched hoare_vcg_if_lift3
-              | simp
-              | strengthen non_kernel_IRQs_strg[where Q=True, simplified], simp cong: conj_cong)+
+                     in hoare_strengthen_postE)
+       apply (wpsimp wp: handle_event_valid_sched)
+      apply simp
+     apply simp
+    apply (wpsimp | strengthen non_kernel_IRQs_strg None_drop)+
    apply (clarsimp simp: active_from_running schact_is_rct_def)
   apply (clarsimp simp: active_from_running')
   done
