proof/refine/ARM_HYP/Syscall_R.thy
@@ -1765,6 +1765,29 @@ lemmas handleReply_ct_in_state_simple[wp] =
     ct_in_state_thread_state_lift' [OF handleReply_ksCurThread
                                      handleReply_st_tcb_at_simple']
 
+lemma handleSpuriousIRQ_corres[corres]:
+  "corres dc \<top> \<top> handle_spurious_irq handleSpuriousIRQ"
+  unfolding handle_spurious_irq_def handleSpuriousIRQ_def
+  by (corres corres: corres_machine_op)
+
+lemma contract_all_imp_strg:
+  "P \<and> P' \<and> (\<forall>x. R x \<longrightarrow> Q x) \<Longrightarrow> \<forall>x. R x \<longrightarrow> P \<and> Q x \<and> P'"
+  by blast
+
+lemma maybeHandleInterrupt_corres:
+  "corres dc einvs invs' (maybe_handle_interrupt in_kernel) (maybeHandleInterrupt in_kernel)"
+  unfolding maybe_handle_interrupt_def maybeHandleInterrupt_def
+  apply (corres corres: corres_machine_op handleInterrupt_corres[@lift_corres_args]
+                simp: irq_state_independent_def
+         | corres_cases_both)+
+     apply (wpsimp wp: hoare_drop_imp)
+    apply clarsimp
+    apply (strengthen contract_all_imp_strg[where P'=True, simplified])
+    apply (wpsimp wp: doMachineOp_getActiveIRQ_IRQ_active' hoare_vcg_all_lift)
+    apply (wpsimp wp: hoare_drop_imp)
+   apply clarsimp
+  apply (clarsimp simp: invs'_def valid_state'_def)
+  done
 
 (* FIXME: move *)
 lemma doReplyTransfer_st_tcb_at_active:
@@ -1947,85 +1970,73 @@ proof -
      apply (clarsimp simp: ct_in_state_def ct_in_state'_def
                      elim!: st_tcb_weakenE pred_tcb'_weakenE)+
     done
-    show ?thesis
-      apply (case_tac event)
-          apply (simp_all add: handleEvent_def)
+  show ?thesis
+    apply (case_tac event)
+         apply (simp_all add: handleEvent_def)
 
-          apply (rename_tac syscall)
-          apply (case_tac syscall)
-          apply (auto intro: corres_guard_imp[OF handleSend_corres]
-                             corres_guard_imp[OF hw]
-                             corres_guard_imp [OF handleReply_corres]
-                             corres_guard_imp[OF handleReply_handleRecv_corres]
-                             corres_guard_imp[OF handleCall_corres]
-                             corres_guard_imp[OF handleYield_corres]
-                             active_from_running active_from_running'
-                      simp: simple_sane_strg)[8]
-         apply (rule corres_underlying_split)
-            apply (rule corres_guard_imp[OF getCurThread_corres], simp+)
-           apply (rule handleFault_corres)
-           apply simp
-          apply (simp add: valid_fault_def)
-          apply wp
-          apply (fastforce elim!: st_tcb_ex_cap st_tcb_weakenE
-                           simp: ct_in_state_def)
-         apply wp
-         apply (clarsimp)
-         apply (auto simp: ct_in_state'_def sch_act_simple_def
-                           sch_act_sane_def
-                     elim: pred_tcb'_weakenE st_tcb_ex_cap'')[1]
+         apply (rename_tac syscall)
+         apply (case_tac syscall)
+                apply (auto intro: corres_guard_imp[OF handleSend_corres]
+                                   corres_guard_imp[OF hw]
+                                   corres_guard_imp [OF handleReply_corres]
+                                   corres_guard_imp[OF handleReply_handleRecv_corres]
+                                   corres_guard_imp[OF handleCall_corres]
+                                   corres_guard_imp[OF handleYield_corres]
+                                   active_from_running active_from_running'
+                            simp: simple_sane_strg)[8]
         apply (rule corres_underlying_split)
-           apply (rule corres_guard_imp, rule getCurThread_corres, simp+)
+           apply (rule corres_guard_imp[OF getCurThread_corres], simp+)
           apply (rule handleFault_corres)
-          apply (simp add: valid_fault_def)
+          apply simp
+         apply (simp add: valid_fault_def)
          apply wp
          apply (fastforce elim!: st_tcb_ex_cap st_tcb_weakenE
-                          simp: ct_in_state_def valid_fault_def)
+                          simp: ct_in_state_def)
         apply wp
-        apply clarsimp
+        apply (clarsimp)
         apply (auto simp: ct_in_state'_def sch_act_simple_def
                           sch_act_sane_def
                     elim: pred_tcb'_weakenE st_tcb_ex_cap'')[1]
-       apply (rule corres_guard_imp)
-         apply (rule corres_split_eqr[where R="\<lambda>rv. einvs"
-                                      and R'="\<lambda>rv s. \<forall>x. rv = Some x \<longrightarrow> R'' x s"
-                                      for R''])
-            apply (rule corres_machine_op)
-            apply (rule corres_Id; wpsimp)
-           apply (case_tac rv, simp_all add: doMachineOp_return)[1]
-           apply (rule handleInterrupt_corres)
-          apply (wp hoare_vcg_all_lift
-                    doMachineOp_getActiveIRQ_IRQ_active'
-                   | simp
-                   | simp add: imp_conjR | wp (once) hoare_drop_imps)+
-       apply (clarsimp simp: invs'_def valid_state'_def ct_not_inQ_def valid_queues_def)
-      apply (rule_tac corres_underlying_split)
-         apply (rule corres_guard_imp, rule getCurThread_corres, simp+)
-        apply (rule corres_split_catch)
-           apply (rule handleVMFault_corres)
-          apply (erule handleFault_corres)
-         apply (wp handle_vm_fault_valid_fault)
-        apply (wp hvmf_invs_etc)
+       apply (rule corres_underlying_split)
+          apply (rule corres_guard_imp, rule getCurThread_corres, simp+)
+         apply (rule handleFault_corres)
+         apply (simp add: valid_fault_def)
+        apply wp
+        apply (fastforce elim!: st_tcb_ex_cap st_tcb_weakenE
+                         simp: ct_in_state_def valid_fault_def)
        apply wp
-       apply (clarsimp simp: simple_from_running tcb_at_invs)
-       apply (fastforce elim!: st_tcb_ex_cap st_tcb_weakenE simp: ct_in_state_def)
+       apply clarsimp
+       apply (auto simp: ct_in_state'_def sch_act_simple_def
+                         sch_act_sane_def
+                   elim: pred_tcb'_weakenE st_tcb_ex_cap'')[1]
+      apply (corres corres: maybeHandleInterrupt_corres)
+     apply (rule_tac corres_underlying_split)
+        apply (rule corres_guard_imp, rule getCurThread_corres, simp+)
+       apply (rule corres_split_catch)
+          apply (rule handleVMFault_corres)
+         apply (erule handleFault_corres)
+        apply (wp handle_vm_fault_valid_fault)
+       apply (wp hvmf_invs_etc)
       apply wp
-      apply (clarsimp)
-      apply (fastforce simp: simple_sane_strg sch_act_simple_def ct_in_state'_def
-                  elim: st_tcb_ex_cap'' pred_tcb'_weakenE)
-         apply (rule corres_underlying_split)
-            apply (rule corres_guard_imp[OF getCurThread_corres], simp+)
-           apply (rule handleHypervisorFault_corres)
-          apply wp
-          apply (fastforce elim!: st_tcb_ex_cap st_tcb_weakenE
-                           simp: ct_in_state_def)
-         apply wp
-         apply (clarsimp)
-         apply (auto simp: ct_in_state'_def sch_act_simple_def
-                           sch_act_sane_def
-                     elim: pred_tcb'_weakenE st_tcb_ex_cap'')[1]
-      done
-  qed
+      apply (clarsimp simp: simple_from_running tcb_at_invs)
+      apply (fastforce elim!: st_tcb_ex_cap st_tcb_weakenE simp: ct_in_state_def)
+     apply wp
+     apply (clarsimp)
+     apply (fastforce simp: simple_sane_strg sch_act_simple_def ct_in_state'_def
+                 elim: st_tcb_ex_cap'' pred_tcb'_weakenE)
+    apply (rule corres_underlying_split)
+       apply (rule corres_guard_imp[OF getCurThread_corres], simp+)
+      apply (rule handleHypervisorFault_corres)
+     apply wp
+     apply (fastforce elim!: st_tcb_ex_cap st_tcb_weakenE
+                      simp: ct_in_state_def)
+    apply wp
+    apply (clarsimp)
+    apply (auto simp: ct_in_state'_def sch_act_simple_def
+                      sch_act_sane_def
+                elim: pred_tcb'_weakenE st_tcb_ex_cap'')[1]
+    done
+qed
 
 crunch handleVMFault
   for st_tcb_at'[wp]: "st_tcb_at' P t"
@@ -2099,6 +2110,27 @@ lemma handleRecv_ksCurThread[wp]:
   "\<lbrace>\<lambda>s. P (ksCurThread s) \<rbrace> handleRecv b \<lbrace>\<lambda>rv s. P (ksCurThread s) \<rbrace>"
   unfolding handleRecv_def
   by ((simp, wp hoare_drop_imps) | wpc | wpsimp wp: hoare_drop_imps)+
+
+lemma handleSpuriousIRQ_invs'[wp]:
+  "handleSpuriousIRQ \<lbrace>invs'\<rbrace>"
+  unfolding handleSpuriousIRQ_def
+  by (wpsimp wp: dmo_invs'_simple)
+
+lemma non_kernel_IRQs_strg:
+  "invs' s \<and> rv \<notin> Some ` non_kernel_IRQs \<and> Q \<Longrightarrow>
+    rv = Some irq \<longrightarrow> invs' s \<and> (irq \<in> non_kernel_IRQs \<longrightarrow> P) \<and> Q"
+  by auto
+
+lemma maybeHandleInterrupt_True_invs'[wp]:
+  "maybeHandleInterrupt True \<lbrace>invs'\<rbrace>"
+  unfolding maybeHandleInterrupt_def
+  by (wpsimp wp: hoare_drop_imp[where Q'="\<lambda>rv _. rv = None"] getActiveIRQ_neq_non_kernel dmo_lift'
+      | strengthen non_kernel_IRQs_strg[where Q=True, simplified])+
+
+lemma maybeHandleInterrupt_False_invs'[wp]:
+  "\<lbrace>\<lambda>s. invs' s \<and> sch_act_not (ksCurThread s) s\<rbrace> maybeHandleInterrupt False \<lbrace>\<lambda>_. invs'\<rbrace>"
+  unfolding maybeHandleInterrupt_def
+  by (wpsimp wp: hoare_drop_imp[where Q'="\<lambda>rv _. rv = None"] hoare_vcg_all_lift hoare_drop_imp)
 
 lemma he_invs'[wp]:
   "\<lbrace>invs' and
